Assign.v
@@ -35,46 +35,46 @@ Record AssnStateInfo := {
 Definition AssnState := State AssnStateInfo.
 
 Definition swapOpM sreg dreg : AssnState (seq opType2) :=
-  assn <-- get ;;[State_Monad]
+  assn <-- get ;;
   let: (mop, acc') := swapOp oinfo sreg dreg (assnAcc assn) in
   put {| assnOpId     := assnOpId assn
        ; assnBlockBeg := assnBlockBeg assn
        ; assnBlockEnd := assnBlockEnd assn
-       ; assnAcc      := acc' |} ;;[State_Monad]
-  pure State_Monad mop.
+       ; assnAcc      := acc' |} ;;
+  pure mop.
 
 Definition moveOpM sreg dreg : AssnState (seq opType2) :=
-  assn <-- get ;;[State_Monad]
+  assn <-- get ;;
   let: (mop, acc') := moveOp oinfo sreg dreg (assnAcc assn) in
   put {| assnOpId     := assnOpId assn
        ; assnBlockBeg := assnBlockBeg assn
        ; assnBlockEnd := assnBlockEnd assn
-       ; assnAcc      := acc' |} ;;[State_Monad]
-  pure State_Monad mop.
+       ; assnAcc      := acc' |} ;;
+  pure mop.
 
 Definition saveOpM vid reg : AssnState (seq opType2) :=
-  assn <-- get ;;[State_Monad]
+  assn <-- get ;;
   let: (sop, acc') := saveOp oinfo vid reg (assnAcc assn) in
   put {| assnOpId     := assnOpId assn
        ; assnBlockBeg := assnBlockBeg assn
        ; assnBlockEnd := assnBlockEnd assn
-       ; assnAcc      := acc' |} ;;[State_Monad]
-  pure State_Monad sop.
+       ; assnAcc      := acc' |} ;;
+  pure sop.
 
 Definition restoreOpM vid reg : AssnState (seq opType2) :=
-  assn <-- get ;;[State_Monad]
+  assn <-- get ;;
   let: (rop, acc') := restoreOp oinfo vid reg (assnAcc assn) in
   put {| assnOpId     := assnOpId assn
        ; assnBlockBeg := assnBlockBeg assn
        ; assnBlockEnd := assnBlockEnd assn
-       ; assnAcc      := acc' |} ;;[State_Monad]
-  pure State_Monad rop.
+       ; assnAcc      := acc' |} ;;
+  pure rop.
 
 Definition pairM {A B : Type} (x : AssnState A) (y : AssnState B) :
   AssnState (A * B)%type :=
-  x' <-- x ;;[State_Monad]
-  y' <-- y ;;[State_Monad]
-  pure State_Monad (x', y').
+  x' <-- x ;;
+  y' <-- y ;;
+  pure (x', y').
 
 Definition varAllocs opid (allocs : seq (Allocation maxReg)) v :
   seq (VarId * PhysReg) :=
@@ -90,57 +90,56 @@ Definition varAllocs opid (allocs : seq (Allocation maxReg)) v :
 
 Definition generateMoves (moves : seq (ResolvingMove maxReg)) :
   AssnState (seq opType2) :=
-  forFoldrM State_Monad [::] moves $ fun mv acc =>
+  forFoldrM [::] moves $ fun mv acc =>
     mops <-- match mv return AssnState (option (seq opType2)) with
-      | Swap    sreg dreg => fmap State_Monad (@Some _) $ swapOpM sreg dreg
-      | Move    sreg dreg => fmap State_Monad (@Some _) $ moveOpM sreg dreg
-      | Spill   sreg vid  => fmap State_Monad (@Some _) $ saveOpM sreg (Some vid)
-      | Restore vid  dreg => fmap State_Monad (@Some _) $ restoreOpM (Some vid) dreg
-      | Nop => pure State_Monad None
-      end ;;[State_Monad]
-    pure State_Monad $ if mops is Some ops then ops ++ acc else acc.
+      | Swap    sreg dreg => fmap (@Some _) $ swapOpM sreg dreg
+      | Move    sreg dreg => fmap (@Some _) $ moveOpM sreg dreg
+      | Spill   sreg vid  => fmap (@Some _) $ saveOpM sreg (Some vid)
+      | Restore vid  dreg => fmap (@Some _) $ restoreOpM (Some vid) dreg
+      | Nop => pure None
+      end ;;
+    pure $ if mops is Some ops then ops ++ acc else acc.
 
 Definition doAllocations (allocs : seq (Allocation maxReg)) op :
   AssnState (seq opType2) :=
-  assn <-- get ;;[State_Monad]
+  assn <-- get ;;
   let opid  := assnOpId assn in
   let vars  := opRefs oinfo op in
-  let regs  := concat (@State_Monad AssnStateInfo) $
-                 map (varAllocs opid allocs) vars in
+  let regs  := concat $ map (varAllocs opid allocs) vars in
   let ops   := applyAllocs oinfo op regs in
 
   transitions <--
     (if assnBlockBeg assn <= opid < assnBlockEnd assn
      then generateMoves
             (determineMoves (resolvingMoves allocs opid opid.+2))
-     else pure State_Monad [::]) ;;[State_Monad]
+     else pure [::]) ;;
 
   (* With lenses, this would just be: assnOpId += 2 *)
-  modify (fun assn' =>
+  modify (fun assn' : AssnStateInfo =>
             {| assnOpId     := opid.+2
              ; assnBlockBeg := assnBlockBeg assn'
              ; assnBlockEnd := assnBlockEnd assn'
-             ; assnAcc      := assnAcc assn' |}) ;;[State_Monad]
+             ; assnAcc      := assnAcc assn' |}) ;;
 
-  pure State_Monad $ ops ++ transitions.
+  pure $ ops ++ transitions.
 
 Definition resolveMappings bid opsm mappings : AssnState (seq opType2) :=
   (* Check whether any boundary transitions require move resolution at the
      beginning or end of the block given by [bid]. *)
-  if IntMap_lookup bid mappings isn't Some graphs then pure State_Monad opsm else
+  if IntMap_lookup bid mappings isn't Some graphs then pure opsm else
 
   let: (gbeg, gend) := graphs in
 
-  bmoves <-- generateMoves (map (@moveFromGraph maxReg) (topsort gbeg)) ;;[State_Monad]
+  bmoves <-- generateMoves (map (@moveFromGraph maxReg) (topsort gbeg)) ;;
   let opsm' := bmoves ++ opsm in
 
-  emoves <-- generateMoves (map (@moveFromGraph maxReg) (topsort gend)) ;;[State_Monad]
+  emoves <-- generateMoves (map (@moveFromGraph maxReg) (topsort gend)) ;;
   let opsm'' := opsm' ++ emoves in
-  pure State_Monad opsm''.
+  pure opsm''.
 
 Definition considerOps (f : opType1 -> AssnState (seq opType2))
   (liveSets : IntMap BlockLiveSets) mappings :=
-  mapM State_Monad $ fun blk =>
+  mapM $ fun blk =>
     (* First apply all allocations *)
     let ops := blockOps binfo blk in
     let bid := blockId binfo blk in
@@ -154,17 +153,17 @@ Definition considerOps (f : opType1 -> AssnState (seq opType2))
               {| assnOpId     := assnOpId assn
                ; assnBlockBeg := assnOpId assn + (size opsb).*2
                ; assnBlockEnd := assnOpId assn + (size opsb + size opsm).*2
-               ; assnAcc      := assnAcc assn |}) ;;[State_Monad]
-    opsb' <-- concatMapM State_Monad f opsb ;;[State_Monad]
-    opsm' <-- concatMapM State_Monad f opsm ;;[State_Monad]
-    opse' <-- concatMapM State_Monad f opse ;;[State_Monad]
+               ; assnAcc      := assnAcc assn |}) ;;
+    opsb' <-- concatMapM f opsb ;;
+    opsm' <-- concatMapM f opsm ;;
+    opse' <-- concatMapM f opse ;;
     (* Insert resolving moves based on the mappings *)
-    opsm'' <-- resolveMappings bid opsm' mappings ;;[State_Monad]
+    opsm'' <-- resolveMappings bid opsm' mappings ;;
     match opsb', opse' with
     | b :: bs, e :: es =>
-        pure State_Monad $ setBlockOps binfo blk
+        pure $ setBlockOps binfo blk
           [:: b] (bs ++ opsm'' ++ belast e es) [:: last e es]
-    | _, _ => pure State_Monad $ setBlockOps binfo blk opsb' opsm'' opse'
+    | _, _ => pure $ setBlockOps binfo blk opsb' opsm'' opse'
     end.
 
 Definition assignRegNum (allocs : seq (Allocation maxReg))
